[repdb] Spec and Proof of the multi-threaded service library.

ml_sources/examples/reliable_communication/lib/mt_server/mt_server_code.ml
@@ -43,5 +43,4 @@ let init_client_proxy
   let skt = make_client_skt ser deser clt_addr in
   let ch = connect skt srv_addr in
   let lk = newlock () in
-  let mk_request req = make_request ch lk req in
-  mk_request
+  make_request ch lk
