aneris/examples/reliable_communication/lib/mt_server/mt_server_code.v
@@ -46,6 +46,4 @@ Definition init_client_proxy ser deser : val :=
   let: "skt" := make_client_skt ser deser "clt_addr" in
   let: "ch" := connect "skt" "srv_addr" in
   let: "lk" := newlock #() in
-  let: "mk_request" := λ: "req",
-  make_request "ch" "lk" "req" in
-  "mk_request".
+  make_request "ch" "lk".
