aneris/examples/reliable_communication/lib/mt_server/spec/api_spec.v
@@ -9,7 +9,8 @@ From aneris.examples.reliable_communication.lib.mt_server
 Section Spec.
   Context `{ !anerisG Mdl Σ, !lockG Σ}.
   Context `{ !MTS_spec_params}.
-  Context ( srv_si : message → iProp Σ).
+  Context (SrvInit : iProp Σ).
+  Context (srv_si : message → iProp Σ).
   Notation srv_ip := (ip_of_address MTS_saddr).
 
 (* Val run_server :
@@ -20,17 +21,19 @@ Section Spec.
        fixed A ∗
        MTS_saddr ⤳ (∅, ∅) ∗
        free_ports (srv_ip) {[port_of_address MTS_saddr]} ∗
+       SrvInit ∗
        is_monitor MTS_mN srv_ip MTS_mγ MTS_mv MTS_mR }}}
      run_server
-        (s_serializer MTS_req_ser)
         (s_serializer MTS_rep_ser)
+        (s_serializer MTS_req_ser)
         #MTS_saddr
         MTS_mv
         MTS_handler
        @[srv_ip]
    {{{ RET #(); ⌜True⌝ }}}.
 
- Definition make_request_spec (handler : val) clt_addr reqv reqd : iProp Σ :=
+ Definition make_request_spec (handler : val) clt_addr : iProp Σ :=
+   ∀ reqv reqd,
    {{{ ⌜Serializable MTS_req_ser reqv⌝ ∗
        MTS_handler_pre reqv reqd }}}
      handler reqv @[ip_of_address clt_addr]
@@ -46,10 +49,10 @@ Section Spec.
      init_client_proxy
         (s_serializer MTS_req_ser)
         (s_serializer MTS_rep_ser)
-        #MTS_saddr
         #sa
+        #MTS_saddr
        @[ip_of_address sa]
-   {{{ reqh, RET reqh; ∀ reqv reqd, make_request_spec reqh sa reqv reqd }}}.
+   {{{ reqh, RET reqh; make_request_spec reqh sa }}}.
 
 End Spec.
 
@@ -59,8 +62,9 @@ Section MTS_Init.
   Class MTS_init := {
     MTS_init_setup E (DLP : MTS_spec_params) :
     ↑MTS_mN ⊆ E →
-    True ⊢ |={E}=> ∃ (srv_si : message → iProp Σ),
-      (∀ A, run_server_spec srv_si A) ∗
+    True ⊢ |={E}=> ∃ (srv_si : message → iProp Σ) (SrvInit : iProp Σ),
+      SrvInit ∗
+      (∀ A, run_server_spec SrvInit srv_si A) ∗
       (∀ A sa, init_client_proxy_spec srv_si A sa) }.
 
 End MTS_Init.
