aneris/examples/reliable_communication/lib/mt_server/proof/mt_server_proof.v
@@ -1,0 +1,284 @@
+From iris.algebra Require Import excl.
+From iris.base_logic.lib Require Import invariants.
+From iris.proofmode Require Import coq_tactics reduction spec_patterns.
+From aneris.aneris_lang Require Import lang.
+From aneris.aneris_lang.lib Require Import lock_proof set_proof.
+From aneris.aneris_lang.lib.serialization Require Import serialization_proof.
+From aneris.aneris_lang Require Import tactics proofmode.
+From actris.channel Require Export proto.
+From aneris.aneris_lang.program_logic Require Import aneris_lifting.
+From aneris.examples.reliable_communication Require Import user_params.
+From aneris.examples.reliable_communication.spec
+     Require Import resources proofmode api_spec.
+From aneris.examples.reliable_communication.lib.mt_server
+     Require Import mt_server_code user_params.
+
+Import mt_server_code.
+Import monitor_proof.
+Import lock_proof.
+Import client_server_code.
+
+Section MTS_proof_of_code.
+  Context `{!anerisG Mdl Σ}.
+  Context `{!lockG Σ}.
+  Context `{!MTS_spec_params}.
+
+  Definition req_prot_aux (rec : iProto Σ)  : iProto Σ :=
+    (<! (reqv : val) (reqd : MTS_req_data) >
+       MSG reqv {{ MTS_handler_pre reqv reqd }} ;
+     <? (repv : val) (repd : MTS_rep_data) >
+       MSG repv {{ MTS_handler_post repv reqd repd }};
+     rec)%proto.
+
+  Instance req_prot_aux_contractive : Contractive (req_prot_aux).
+  Proof. solve_proto_contractive. Qed.
+  Definition req_prot : iProto Σ := fixpoint (req_prot_aux).
+  Global Instance req_prot_unfold :
+    ProtoUnfold req_prot (req_prot_aux req_prot).
+  Proof. apply proto_unfold_eq, fixpoint_unfold. Qed.
+
+  Global Instance MT_UP : Reliable_communication_service_params :=
+  {| RCParams_clt_ser := MTS_req_ser;
+     RCParams_srv_ser := MTS_rep_ser;
+     RCParams_srv_ser_inj := MTS_rep_ser_inj;
+     RCParams_srv_ser_inj_alt := MTS_rep_ser_inj_alt;
+     RCParams_clt_ser_inj := MTS_req_ser_inj;
+     RCParams_clt_ser_inj_alt := MTS_req_ser_inj_alt;
+     RCParams_srv_saddr := MTS_saddr;
+     RCParams_protocol := req_prot;
+     RCParams_srv_N := MTS_mN;
+  |}.
+
+  Context `{cmh: !@Chan_mapsto_resource Σ}.
+  Context `{SnRes : !SessionResources MT_UP}.
+  Context `{HspecS : !Reliable_communication_Specified_API_session cmh}.
+  Context `{HspecN : !Reliable_communication_Specified_API_network MT_UP SnRes}.
+
+  Lemma service_loop_proof (c : val) :
+    {{{ is_monitor MTS_mN (ip_of_address MTS_saddr) MTS_mγ MTS_mv MTS_mR ∗
+        c ↣{ ip_of_address MTS_saddr, MTS_rep_ser } iProto_dual req_prot  }}}
+      service_loop c MTS_mv MTS_handler #() @[ip_of_address MTS_saddr]
+    {{{ RET #(); ⌜True⌝  }}}.
+  Proof.
+    iIntros (Φ) "(#Hlk & Hc) HΦ". rewrite /service_loop.
+    do 10 wp_pure _.
+    iLöb as "IH".
+    wp_pures.
+    rewrite /req_prot. rewrite /req_prot_aux.
+    simpl in *.
+    wp_recv (reqv reqd) as "HreqPre".
+    wp_pures.
+    wp_apply (monitor_acquire_spec with "[Hlk]"); first by iFrame "#".
+    iIntros (v) "(-> & HKey & HR)".
+    wp_pures.
+    wp_apply (MTS_handler_spec with "[$Hlk $HKey $HR $HreqPre]").
+    iIntros (repv repd) "(%Hser & HKey & HR & HreqPost)".
+    wp_pures.
+    wp_apply (monitor_release_spec with "[$Hlk $HR $HKey]").
+    iIntros (v ->).
+    do 2 wp_pure _.
+    wp_send with "[$HreqPost]".
+    do 2 wp_pure _.
+    by iApply ("IH" with "[$Hc]").
+  Qed.
+
+  Lemma wp_accept_new_connections_loop skt  :
+    {{{ MTS_saddr ⤇ reserved_server_socket_interp ∗
+        SrvListens skt ∗
+        is_monitor MTS_mN (ip_of_address MTS_saddr) MTS_mγ MTS_mv MTS_mR }}}
+      accept_new_connections_loop skt MTS_mv MTS_handler #()
+      @[ip_of_address RCParams_srv_saddr]
+    {{{ RET #(); False }}}.
+  Proof.
+    iIntros (Φ) "(#Hsi & Hlistens & #Hlk) HΦ".
+    rewrite /accept_new_connections_loop.
+    do 10 (wp_pure _).
+    iLöb as "IH".
+    wp_pure _.
+    wp_smart_apply (RCSpec_accept_spec with "[$Hlistens]").
+    iIntros (c clt_addr v) "(-> & Hlistens & Hc)".
+    wp_pures.
+    wp_apply (aneris_wp_fork with "[-]").
+    iSplitL "Hlistens".
+    - iNext.
+      do 2 wp_pure _.
+      iApply ("IH" with "[$Hlistens]").
+      by iIntros.
+    - iNext.
+      wp_pures.
+      simpl in *.
+      by wp_apply (service_loop_proof with "[$Hlk $Hc]").
+  Qed.
+
+  Definition run_server_internal_spec A : iProp Σ :=
+    {{{ ⌜MTS_saddr ∈ A⌝ ∗
+        fixed A ∗
+        free_ports (ip_of_address MTS_saddr) {[port_of_address MTS_saddr]} ∗
+        MTS_saddr ⤇ reserved_server_socket_interp ∗
+        MTS_saddr ⤳ (∅, ∅) ∗
+        SrvInit ∗
+        is_monitor MTS_mN (ip_of_address MTS_saddr) MTS_mγ MTS_mv MTS_mR }}}
+      run_server
+        (s_serializer MTS_rep_ser)
+        (s_serializer MTS_req_ser)
+        #MTS_saddr
+        MTS_mv
+        MTS_handler
+        @[ip_of_address MTS_saddr]
+    {{{ RET #(); ⌜True⌝ }}}.
+
+  Lemma run_server_internal_spec_holds A : ⊢ run_server_internal_spec A.
+  Proof.
+    iIntros (Φ) "!#".
+    iIntros "Hres HΦ".
+    iDestruct "Hres" as "(#HA & #Hf & Hfp & #Hsi & Hmh & Hinit & #Hmon)".
+    rewrite /run_server.
+    wp_pures.
+    wp_apply (RCSpec_make_server_skt_spec with "[$HA $Hmh $Hsi $Hf $Hinit $Hfp][HΦ]").
+    iNext. iIntros (skt) "Hcl".
+    wp_pures.
+    wp_apply (RCSpec_server_listen_spec with "[$Hcl][HΦ]").
+    iNext. iIntros (v) "(-> & Hp)".
+    wp_pures.
+    wp_apply aneris_wp_fork.
+    iSplitL "HΦ".
+    - iNext; by iApply "HΦ".
+    - by iApply (wp_accept_new_connections_loop with "[$]").
+  Qed.
+
+  Definition make_request_spec_internal (handler : val) clt_addr : iProp Σ :=
+    ∀ reqv reqd,
+    {{{ ⌜Serializable MTS_req_ser reqv⌝ ∗ MTS_handler_pre reqv reqd }}}
+      handler reqv @[ip_of_address clt_addr]
+    {{{ repd repv, RET repv; MTS_handler_post repv reqd repd  }}}.
+
+  Lemma make_request_spec_internal_holds c lk γlk sa :
+    {{{  is_lock (MTS_mN.@"proxy") (ip_of_address sa) γlk lk
+            (c ↣{ip_of_address sa,RCParams_clt_ser} RCParams_protocol) }}}
+      make_request c lk @[ip_of_address sa]
+    {{{ reqh, RET reqh; make_request_spec_internal reqh sa }}}.
+  Proof.
+    iIntros (Φ) "#Hlk HΦ".
+    rewrite /make_request.
+    wp_pures.
+    iApply "HΦ".
+    rewrite /make_request_spec_internal.
+    iIntros (reqv reqd) "!#".
+    iIntros (Ψ) "(%Hser & HreqPre) HΨ".
+    wp_pures.
+    wp_apply (acquire_spec with "[$Hlk]").
+    iIntros (v) "(-> & HKey & HR)".
+    wp_pures.
+    wp_send with "[$HreqPre]".
+    wp_pures.
+    wp_recv (repv repd) as "HreqPost".
+    wp_pures.
+    wp_apply (release_spec with "[$Hlk $HR $HKey]").
+    iIntros (v ->).
+    wp_pures.
+    by iApply "HΨ".
+  Qed.
+
+  Definition init_client_proxy_internal_spec A sa : iProp Σ :=
+    {{{ ⌜sa ∉ A⌝ ∗
+        fixed A ∗
+        free_ports (ip_of_address sa) {[port_of_address sa]} ∗ sa ⤳ (∅, ∅) ∗
+        MTS_saddr ⤇ reserved_server_socket_interp }}}
+      init_client_proxy
+        (s_serializer MTS_req_ser)
+        (s_serializer MTS_rep_ser)
+        #sa
+        #MTS_saddr
+       @[ip_of_address sa]
+    {{{ reqh, RET reqh; make_request_spec_internal reqh sa }}}.
+
+  Lemma init_client_proxy_internal_spec_holds A sa : ⊢ init_client_proxy_internal_spec A sa.
+  Proof.
+    iIntros (Φ) "!#".
+    iIntros "(#HnA & #Hf & Hfp & Hmh & #Hsi) HΦ".
+    rewrite /init_client_proxy.
+    wp_pures.
+    wp_apply (RCSpec_make_client_skt_spec with "[$HnA $Hmh $Hsi $Hf $Hfp][HΦ]").
+    iNext.
+    iIntros (skt) "Hcl".
+    wp_pures.
+    wp_apply (RCSpec_connect_spec with "[$Hcl][HΦ]").
+    iNext. iIntros (c) "Hcl". wp_pures.
+    wp_apply (newlock_spec
+                (MTS_mN .@ "proxy") _
+                ( c ↣{ip_of_address sa,RCParams_clt_ser} RCParams_protocol) with "[$Hcl]").
+    iIntros (lk γlk) "#Hlk".
+    wp_pures.
+    by wp_apply (make_request_spec_internal_holds c lk γlk with "[$Hlk]").
+  Qed.
+
+End MTS_proof_of_code.
+
+From aneris.examples.reliable_communication.lib.mt_server.spec Require Import api_spec.
+
+Section MTS_proof_of_init.
+  Context `{!anerisG Mdl Σ}.
+  Context `{!lockG Σ}.
+  Context `{!MTS_spec_params}.
+  Context `{!Reliable_communication_init}.
+
+  Lemma MTS_init_setup_holds (E : coPset) :
+    ↑MTS_mN ⊆ E →
+    True ⊢ |={E}=> ∃ (srv_si : message → iProp Σ) (SrvInit : iProp Σ),
+      SrvInit ∗
+      (∀ A, run_server_spec SrvInit srv_si A) ∗
+      (∀ A sa, init_client_proxy_spec srv_si A sa).
+  Proof.
+    iIntros (HE _).
+    iMod (Reliable_communication_init_setup E MT_UP HE $! ⊤)
+      as (chn sgn) "(Hinit & Hspecs)".
+    iDestruct "Hspecs"
+      as "(
+           %HmkClt & %HmkSrv
+         & %Hconnect
+         & %Hlisten & %Haccept
+         & %Hsend & %HsendTele
+         & %HtryRecv & %Hrecv)".
+    Unshelve. 2: { done. }
+    iExists reserved_server_socket_interp, SrvInit.
+    iFrame.
+    iModIntro.
+    iSplitL.
+    - iIntros (A Φ) "!#".
+      iIntros "(#Hsi & HinA & Hf & Hmh & Hfp & Hinit & #Hmon) HΦ".
+      iDestruct run_server_internal_spec_holds as "#HserviceSpec".
+      iApply ("HserviceSpec" with "[$HinA $Hf $Hfp $Hsi $Hmon $Hmh $Hinit][$]").
+      Unshelve.
+      + done.
+      + split; done.
+      + split; done.
+    - iIntros (A sa Φ) "!#".
+      iIntros "(HinA & Hf & Hfp & Hmh & #Hsi) HΦ".
+      iDestruct (init_client_proxy_internal_spec_holds) as "#HclientSpec".
+      by iApply ("HclientSpec" with "[$HinA $Hf $Hfp $Hmh $Hsi][HΦ]").
+      Unshelve.
+      + done.
+      + split; try done.
+      + split; try done.
+  Qed.
+
+
+End MTS_proof_of_init.
+
+Section MTS_proof_of_the_init_class.
+  Context `{!anerisG Mdl Σ}.
+  Context `{!lockG Σ}.
+  Context `{!MTS_spec_params}.
+  Context `{!Reliable_communication_init}.
+
+  Global Instance mts_init : MTS_init.
+  Proof.
+    split. iIntros (E MTS_sps HE _).
+    iMod (MTS_init_setup_holds E HE $! ⊤) as  (srv_si SrvInit) "(Ha & Hb & Hc)".
+    iModIntro.
+    iExists _, _.
+    iFrame.
+    Unshelve. done.
+  Qed.
+
+End MTS_proof_of_the_init_class.
